SP1Clean/Proofs/Chips/ShiftRightChip/Soundness/Sraw.lean
@@ -367,9 +367,9 @@ theorem soundness : GeneralFormalCircuit.Soundness (ZMod p) main Assumptions Spe
             exact a2eq
           · show env.get (i₀ + 3) = srwmsb * 65535
             exact a3eq
-          · show (ShiftRightMath.HWord.toBitVec32 #v[env.get i₀, env.get (i₀ + 1)]).toNat
+          · show (HWord.toBitVec32 #v[env.get i₀, env.get (i₀ + 1)]).toNat
                 = 2 ^ 32 - 1 - (2 ^ 32 - 1
-                    - (ShiftRightMath.HWord.toBitVec32 #v[input_adapter_op_b_memory_prev_value[0],
+                    - (HWord.toBitVec32 #v[input_adapter_op_b_memory_prev_value[0],
                         input_adapter_op_b_memory_prev_value[1]]).toNat)
                     / 2 ^ (input_adapter_op_c_memory_prev_value[0].val % 32)
             rw [ha0, ha1, eq_lr0, eq_lr1, h_ll2_0, zero_mul, add_zero, h_c0mod32]
@@ -415,9 +415,9 @@ theorem soundness : GeneralFormalCircuit.Soundness (ZMod p) main Assumptions Spe
             exact a2eq
           · show env.get (i₀ + 3) = srwmsb * 65535
             exact a3eq
-          · show (ShiftRightMath.HWord.toBitVec32 #v[env.get i₀, env.get (i₀ + 1)]).toNat
+          · show (HWord.toBitVec32 #v[env.get i₀, env.get (i₀ + 1)]).toNat
                 = 2 ^ 32 - 1 - (2 ^ 32 - 1
-                    - (ShiftRightMath.HWord.toBitVec32 #v[input_adapter_op_b_memory_prev_value[0],
+                    - (HWord.toBitVec32 #v[input_adapter_op_b_memory_prev_value[0],
                         input_adapter_op_b_memory_prev_value[1]]).toNat)
                     / 2 ^ (input_adapter_op_c_memory_prev_value[0].val % 32)
             rw [ha0, ha1, eq_lr1, h_ll2_0, zero_mul, add_zero, h_c0mod32]
@@ -472,8 +472,8 @@ theorem soundness : GeneralFormalCircuit.Soundness (ZMod p) main Assumptions Spe
             exact a2eq
           · show env.get (i₀ + 3) = srwmsb * 65535
             exact a3eq
-          · show (ShiftRightMath.HWord.toBitVec32 #v[env.get i₀, env.get (i₀ + 1)]).toNat
-                = (ShiftRightMath.HWord.toBitVec32 #v[input_adapter_op_b_memory_prev_value[0],
+          · show (HWord.toBitVec32 #v[env.get i₀, env.get (i₀ + 1)]).toNat
+                = (HWord.toBitVec32 #v[input_adapter_op_b_memory_prev_value[0],
                     input_adapter_op_b_memory_prev_value[1]]).toNat
                   / 2 ^ (input_adapter_op_c_memory_prev_value[0].val % 32)
             rw [ha0, ha1, eq_lr0, eq_lr1, h_ll2_0, zero_mul, add_zero, h_c0mod32]
@@ -519,8 +519,8 @@ theorem soundness : GeneralFormalCircuit.Soundness (ZMod p) main Assumptions Spe
             exact a2eq
           · show env.get (i₀ + 3) = srwmsb * 65535
             exact a3eq
-          · show (ShiftRightMath.HWord.toBitVec32 #v[env.get i₀, env.get (i₀ + 1)]).toNat
-                = (ShiftRightMath.HWord.toBitVec32 #v[input_adapter_op_b_memory_prev_value[0],
+          · show (HWord.toBitVec32 #v[env.get i₀, env.get (i₀ + 1)]).toNat
+                = (HWord.toBitVec32 #v[input_adapter_op_b_memory_prev_value[0],
                     input_adapter_op_b_memory_prev_value[1]]).toNat
                   / 2 ^ (input_adapter_op_c_memory_prev_value[0].val % 32)
             rw [ha0, ha1, eq_lr1, h_ll2_0, zero_mul, add_zero, h_c0mod32]
